ReadMe.md
@@ -5,3 +5,7 @@ enum all terms of size n
 for each term l:
 synthesize kbo minimal term r, add rule l -> r
 
+
+Alg 1:
+Simplify with R n, if smaller size, discard
+otherwise: smt
